src/program_proof/pav/history.v
@@ -16,3 +16,48 @@ Definition own (ptr : loc) (obj : t) : iProp Σ :=
   "#Hsl_HistVal" ∷ own_slice_small sl_HistVal byteT DfracDiscarded obj.(HistVal).
 End defs.
 End HistEntry.
+
+(* logical history. this may be the same as the physical history.
+but lets leave it abstract for now, so we can fill in details later
+once we know the use case. *)
+Module hist.
+Definition t : Type. Admitted.
+(* TODO: the core invariant about the logical history. *)
+Definition inv (obj : t) : Prop. Admitted.
+(* relation bw physical and logical st.  *)
+Definition phys_relate (obj : t) (hist : list HistEntry.t) : Prop. Admitted.
+End hist.
+
+Section defs.
+Context `{!heapGS Σ}.
+Definition own_hist sl_hist (hist : list HistEntry.t) : iProp Σ :=
+  ∃ dim0_hist,
+  "Hsl_hist" ∷ own_slice sl_hist ptrT (DfracOwn 1) dim0_hist ∗
+  "Hdim0_hist" ∷ ([∗ list] p;o ∈ dim0_hist;hist, HistEntry.own p o) ∗
+  "Hrelate" ∷ hist.phys_relate log_hist hist ∗
+  "Hhist_inv" ∷ inv hist.
+End defs.
+
+Section wps.
+Context `{!heapGS Σ}.
+Lemma wp_GetHist sl_hist hist (epoch : w64) :
+  {{{
+    "Hown_hist" ∷ own_hist sl_hist hist
+  }}}
+  GetHist (slice_val sl_hist) #epoch
+  {{{
+    (is_reg : bool) sl_lat_val (lat_val : list w8), RET (#is_reg, slice_val sl_lat_val);
+    (* could directly say that lat_val is an element in the hist that corresponds to the max epoch
+    less than the one queried. *)
+    (* or, could say that the output matches whatever is returned by some logical object.
+    ultimately, it's prob easier to reason about the logical object with other things,
+    e.g., msv's, so let's have the output match that. *)
+    (* secondly, what logical state do we wanna use?
+    before, i explicitly made the logical object basically the same thing.
+    and i made the get fn something.
+    can i be more abstract here?
+    there exists some logical object, and this thing is tied into it.
+    and that object has a get fn.
+    *)
+  }}}.
+End wps.
